Remove inp from locale

Earley_List.thy
@@ -70,22 +70,22 @@ definition wf_bins :: "'a rules \<Rightarrow> 'a list \<Rightarrow> 'a bins \<Ri
 typedef 'a wf_bins = "{ (bs::'a bins) | \<RR> inp bs. wf_bins \<RR> inp bs }"
   sorry
 
-locale Earley_List = Earley_Set +
+locale Earley = CFG +
   assumes distinct_rules: "distinct \<RR>"
   assumes nonempty_deriv: "N \<in> set \<NN> \<Longrightarrow> \<not> derives [N] []"
 begin
 
 subsection \<open>Earley algorithm\<close>
 
-definition Init_it :: "'a bins" where
-  "Init_it = (
+definition Init_it :: "'a sentence \<Rightarrow> 'a bins" where
+  "Init_it inp = (
     let rs = filter (\<lambda>r. rule_head r = \<SS>) \<RR> in
     let b0 = map (\<lambda>r. init_item r 0) rs in
     let bs = replicate (length inp + 1) (Bin []) in
     app_bins (Bins bs) 0 b0)"
 
-definition Scan_it :: "nat \<Rightarrow> 'a  \<Rightarrow> 'a item \<Rightarrow> 'a item list" where
-  "Scan_it k a x = (
+definition Scan_it :: "nat \<Rightarrow> 'a sentence \<Rightarrow> 'a  \<Rightarrow> 'a item \<Rightarrow> 'a item list" where
+  "Scan_it k inp a x = (
     if k < length inp \<and> inp!k = a then
       let x' = inc_item x (k+1) in
       [x']
@@ -106,8 +106,8 @@ lemma wf_bins_kth_bin:
   "wf_bins \<RR> inp bs \<Longrightarrow> k < length (bins bs) \<Longrightarrow> x \<in> set_bin (bins bs ! k) \<Longrightarrow> wf_item \<RR> inp x \<and> item_end x = k"
   using set_bin_def wf_bin_def wf_bins_def by blast
 
-function \<pi>_it' :: "nat \<Rightarrow> 'a bins \<Rightarrow> nat \<Rightarrow> 'a bins" where
-  "\<pi>_it' k bs i = (
+function \<pi>_it' :: "nat \<Rightarrow> 'a sentence \<Rightarrow> 'a bins \<Rightarrow> nat \<Rightarrow> 'a bins" where
+  "\<pi>_it' k inp bs i = (
     if k \<ge> length (bins bs) \<or> \<not> wf_bins \<RR> inp bs \<or> i \<ge> length (items (bins bs ! k)) then bs
     else
       let x = items (bins bs!k) ! i in
@@ -115,18 +115,18 @@ function \<pi>_it' :: "nat \<Rightarrow> 'a bins \<Rightarrow> nat \<Rightarrow>
         case next_symbol x of
           Some a \<Rightarrow>
             if is_terminal a then
-              if k < length inp then app_bins bs (k+1) (Scan_it k a x)
+              if k < length inp then app_bins bs (k+1) (Scan_it k inp a x)
               else bs
             else app_bins bs k (Predict_it k a)
         | None \<Rightarrow> app_bins bs k (Complete_it k x bs)
-      in \<pi>_it' k bs' (i+1))"
+      in \<pi>_it' k inp bs' (i+1))"
   by pat_completeness simp
 termination
-  apply (relation "measure (\<lambda>(k,bs,i). card { x | x. wf_item \<RR> inp x \<and> item_end x = k } - i)")
+  apply (relation "measure (\<lambda>(k,inp,bs,i). card { x | x. wf_item \<RR> inp x \<and> item_end x = k } - i)")
   apply auto
-  subgoal premises prems for k bs i
+  subgoal premises prems for k inp bs i
   proof -
-    have 0:  "set (items (bins bs ! k)) \<subseteq> { x | x. wf_item \<RR> inp x \<and> item_end x = k }"
+    have 0: "set (items (bins bs ! k)) \<subseteq> { x | x. wf_item \<RR> inp x \<and> item_end x = k }"
       using prems(1,2) not_le_imp_less wf_bins_kth_bin by fastforce
     have 1: "finite { x | x. wf_item \<RR> inp x \<and> item_end x = k }"
       using finiteness_UNIV_wf_item by simp
@@ -143,51 +143,51 @@ termination
   qed
   done
 
-definition \<pi>_it :: "nat \<Rightarrow> 'a bins \<Rightarrow> 'a bins" where
-  "\<pi>_it k bs = \<pi>_it' k bs 0"
+definition \<pi>_it :: "nat \<Rightarrow> 'a sentence \<Rightarrow> 'a bins \<Rightarrow> 'a bins" where
+  "\<pi>_it k inp bs = \<pi>_it' k inp bs 0"
 
-fun \<I>_it :: "nat \<Rightarrow> 'a bins" where
-  "\<I>_it 0 = \<pi>_it 0 Init_it"
-| "\<I>_it (Suc n) = \<pi>_it (Suc n) (\<I>_it n)"
+fun \<I>_it :: "nat \<Rightarrow> 'a sentence \<Rightarrow> 'a bins" where
+  "\<I>_it 0 inp = \<pi>_it 0 inp (Init_it inp)"
+| "\<I>_it (Suc n) inp = \<pi>_it (Suc n) inp (\<I>_it n inp)"
 
-definition \<II>_it :: "'a bins" where
-  "\<II>_it = \<I>_it (length inp)"
+definition \<II>_it :: "'a sentence \<Rightarrow> 'a bins" where
+  "\<II>_it inp = \<I>_it (length inp) inp"
 
 subsubsection \<open>Alternate \<pi>_it' simps and induction rule\<close>
 
 lemma \<pi>_it'_simps[simp]:
-  "k \<ge> length (bins bs) \<or> \<not> wf_bins \<RR> inp bs \<or> i \<ge> length (items (bins bs ! k)) \<Longrightarrow> \<pi>_it' k bs i = bs"
+  "k \<ge> length (bins bs) \<or> \<not> wf_bins \<RR> inp bs \<or> i \<ge> length (items (bins bs ! k)) \<Longrightarrow> \<pi>_it' k inp bs i = bs"
   "\<not> (k \<ge> length (bins bs) \<or> \<not> wf_bins \<RR> inp bs \<or> i \<ge> length (items (bins bs ! k))) \<Longrightarrow> 
     x = items (bins bs!k) ! i \<Longrightarrow> next_symbol x = None \<Longrightarrow>
-    \<pi>_it' k bs i = \<pi>_it' k (app_bins bs k (Complete_it k x bs)) (i+1)"
+    \<pi>_it' k inp bs i = \<pi>_it' k inp (app_bins bs k (Complete_it k x bs)) (i+1)"
   "\<not> (k \<ge> length (bins bs) \<or> \<not> wf_bins \<RR> inp bs \<or> i \<ge> length (items (bins bs ! k))) \<Longrightarrow>
     x = items (bins bs!k) ! i \<Longrightarrow> next_symbol x = Some a \<Longrightarrow> is_terminal a \<Longrightarrow> k < length inp \<Longrightarrow>
-    \<pi>_it' k bs i = \<pi>_it' k (app_bins bs (k+1) (Scan_it k a x)) (i+1)"
+    \<pi>_it' k inp bs i = \<pi>_it' k inp (app_bins bs (k+1) (Scan_it k inp a x)) (i+1)"
   "\<not> (k \<ge> length (bins bs) \<or> \<not> wf_bins \<RR> inp bs \<or> i \<ge> length (items (bins bs ! k))) \<Longrightarrow>
      x = items (bins bs!k) ! i \<Longrightarrow> next_symbol x = Some a \<Longrightarrow> is_terminal a \<Longrightarrow> \<not> k < length inp \<Longrightarrow>
-    \<pi>_it' k bs i = \<pi>_it' k bs (i+1)"
+    \<pi>_it' k inp bs i = \<pi>_it' k inp bs (i+1)"
   "\<not> (k \<ge> length (bins bs) \<or> \<not> wf_bins \<RR> inp bs \<or> i \<ge> length (items (bins bs ! k))) \<Longrightarrow>
      x = items (bins bs!k) ! i \<Longrightarrow> next_symbol x = Some a \<Longrightarrow> \<not> is_terminal a \<Longrightarrow>
-    \<pi>_it' k bs i = \<pi>_it' k (app_bins bs k (Predict_it k a)) (i+1)"
+    \<pi>_it' k inp bs i = \<pi>_it' k inp (app_bins bs k (Predict_it k a)) (i+1)"
   by (simp_all, simp_all add: Let_def)
 
 lemma \<pi>_it'_induct[case_names Base Complete Scan Pass Predict]:
-  assumes base: "\<And>k bs i. k \<ge> length (bins bs) \<or> \<not> wf_bins \<RR> inp bs \<or> i \<ge> length (items (bins bs ! k)) \<Longrightarrow> P k bs i"
-  assumes complete: "\<And>k bs i x. \<not> (k \<ge> length (bins bs) \<or> \<not> wf_bins \<RR> inp bs \<or> i \<ge> length (items (bins bs ! k))) \<Longrightarrow>
+  assumes base: "\<And>k inp bs i. k \<ge> length (bins bs) \<or> \<not> wf_bins \<RR> inp bs \<or> i \<ge> length (items (bins bs ! k)) \<Longrightarrow> P k inp bs i"
+  assumes complete: "\<And>k inp bs i x. \<not> (k \<ge> length (bins bs) \<or> \<not> wf_bins \<RR> inp bs \<or> i \<ge> length (items (bins bs ! k))) \<Longrightarrow>
             x = items (bins bs ! k) ! i \<Longrightarrow> next_symbol x = None \<Longrightarrow> (\<And>xa. xa = app_bins bs k (Complete_it k x bs) \<Longrightarrow>
-            P k xa (i+1)) \<Longrightarrow> P k bs i"
-  assumes scan: "\<And>k bs i x a. \<not> (k \<ge> length (bins bs) \<or> \<not> wf_bins \<RR> inp bs \<or> i \<ge> length (items (bins bs ! k))) \<Longrightarrow>
+            P k inp xa (i+1)) \<Longrightarrow> P k inp bs i"
+  assumes scan: "\<And>k inp bs i x a. \<not> (k \<ge> length (bins bs) \<or> \<not> wf_bins \<RR> inp bs \<or> i \<ge> length (items (bins bs ! k))) \<Longrightarrow>
             x = items (bins bs ! k) ! i \<Longrightarrow> next_symbol x = Some a \<Longrightarrow> is_terminal a \<Longrightarrow> k < length inp \<Longrightarrow> 
-            (\<And>xa. xa = app_bins bs (k+1) (Scan_it k a x) \<Longrightarrow> P k xa (i+1)) \<Longrightarrow> P k bs i"
-  assumes pass: "\<And>k bs i x a. \<not> (k \<ge> length (bins bs) \<or> \<not> wf_bins \<RR> inp bs \<or> i \<ge> length (items (bins bs ! k))) \<Longrightarrow>
+            (\<And>xa. xa = app_bins bs (k+1) (Scan_it k inp a x) \<Longrightarrow> P k inp xa (i+1)) \<Longrightarrow> P k inp bs i"
+  assumes pass: "\<And>k inp bs i x a. \<not> (k \<ge> length (bins bs) \<or> \<not> wf_bins \<RR> inp bs \<or> i \<ge> length (items (bins bs ! k))) \<Longrightarrow>
             x = items (bins bs ! k) ! i \<Longrightarrow> next_symbol x = Some a \<Longrightarrow> is_terminal a \<Longrightarrow> \<not> k < length inp \<Longrightarrow>
-            P k bs (i+1) \<Longrightarrow> P k bs i"
-  assumes predict: "\<And>k bs i x a. \<not> (k \<ge> length (bins bs) \<or> \<not> wf_bins \<RR> inp bs \<or> i \<ge> length (items (bins bs ! k))) \<Longrightarrow>
+            P k inp bs (i+1) \<Longrightarrow> P k inp bs i"
+  assumes predict: "\<And>k inp bs i x a. \<not> (k \<ge> length (bins bs) \<or> \<not> wf_bins \<RR> inp bs \<or> i \<ge> length (items (bins bs ! k))) \<Longrightarrow>
             x = items (bins bs ! k) ! i \<Longrightarrow> next_symbol x = Some a \<Longrightarrow> \<not> is_terminal a \<Longrightarrow> 
-            (\<And>xa. xa = app_bins bs k (Predict_it k a) \<Longrightarrow> P k xa (i+1)) \<Longrightarrow> P k bs i"
-  shows "P k bs i"
-proof (induction k bs i rule: \<pi>_it'.induct)
-  case (1 k bs i)
+            (\<And>xa. xa = app_bins bs k (Predict_it k a) \<Longrightarrow> P k inp xa (i+1)) \<Longrightarrow> P k inp bs i"
+  shows "P k inp bs i"
+proof (induction k inp bs i rule: \<pi>_it'.induct)
+  case (1 k inp bs i)
   show ?case
   proof cases
     assume "k \<ge> length (bins bs) \<or> \<not> wf_bins \<RR> inp bs \<or> i \<ge> length (items (bins bs ! k))"
@@ -244,7 +244,7 @@ lemma length_nth_bin_app_bins_eq:
   by (cases "k < length (bins bs)") (auto simp: app_bins_def app_bin_def)
 
 lemma length_bins_Init_it[simp]:
-  "length (bins Init_it) = length inp + 1"
+  "length (bins (Init_it inp)) = length inp + 1"
   unfolding Init_it_def using length_bins_app_bins by force
 
 lemma app_bins_eq:
@@ -316,27 +316,27 @@ lemma distinct_app_bins:
   unfolding app_bins_def by (auto, metis distinct_app_bin list_update_beyond not_le_imp_less nth_list_update_eq)
 
 lemma length_bins_\<pi>_it'[simp]:
-  "length (bins (\<pi>_it' k bs i)) = length (bins bs)"
-  by (induction k bs i rule: \<pi>_it'_induct) auto
+  "length (bins (\<pi>_it' k inp bs i)) = length (bins bs)"
+  by (induction k inp bs i rule: \<pi>_it'_induct) auto
 
 lemma length_bins_\<pi>_it[simp]:
-  "length (bins (\<pi>_it k bs)) = length (bins bs)"
+  "length (bins (\<pi>_it k inp bs)) = length (bins bs)"
   unfolding \<pi>_it_def by simp
 
 lemma length_nth_bin_\<pi>_it':
-  "length (items (bins (\<pi>_it' k bs i) ! l)) \<ge> length (items (bins bs ! l))"
+  "length (items (bins (\<pi>_it' k inp bs i) ! l)) \<ge> length (items (bins bs ! l))"
   using length_nth_bin_app_bins order_trans
-  by (induction k bs i rule: \<pi>_it'_induct) (auto, blast+)
+  by (induction k inp bs i rule: \<pi>_it'_induct) (auto, blast+)
 
 lemma length_bins_\<I>_it[simp]:
-  "length (bins (\<I>_it k)) = length (bins Init_it)"
+  "length (bins (\<I>_it k inp)) = length (bins (Init_it inp))"
   by (induction k) auto
 
 lemma kth_\<pi>_it'_bins:
   assumes "j < length (items (bins bs ! l))"
-  shows "items (bins (\<pi>_it' k bs i) ! l) ! j = items (bins bs ! l) ! j"
+  shows "items (bins (\<pi>_it' k inp bs i) ! l) ! j = items (bins bs ! l) ! j"
   using assms length_nth_bin_app_bins nth_app_bins kth_app_bins length_bins_app_bins
-  apply (induction k bs i rule: \<pi>_it'_induct)
+  apply (induction k inp bs i rule: \<pi>_it'_induct)
   apply (auto)
   apply (smt (verit) Orderings.preorder_class.dual_order.trans Suc_le_eq kth_app_bins length_nth_bin_app_bins nth_app_bins)
   apply (smt (verit, best) length_nth_bin_app_bins kth_app_bins nth_app_bins order_less_le_trans)
@@ -344,26 +344,26 @@ lemma kth_\<pi>_it'_bins:
 
 lemma nth_bin_sub_\<pi>_it':
   assumes "k < length (bins bs)" "l < length (bins bs)"
-  shows "set_bin (bins bs ! l) \<subseteq> set_bin (bins (\<pi>_it' k bs i) ! l)"
+  shows "set_bin (bins bs ! l) \<subseteq> set_bin (bins (\<pi>_it' k inp bs i) ! l)"
 proof standard
   fix x
   assume "x \<in> set_bin (bins bs ! l)"
   then obtain j where *: "j < length (items (bins bs ! l))" "items (bins bs ! l) ! j = x"
     using set_bin_def in_set_conv_nth by metis
-  have "x = items (bins (\<pi>_it' k bs i) ! l) ! j"
+  have "x = items (bins (\<pi>_it' k inp bs i) ! l) ! j"
     using kth_\<pi>_it'_bins assms * by simp
-  moreover have "j < length (items (bins (\<pi>_it' k bs i) ! l))"
+  moreover have "j < length (items (bins (\<pi>_it' k inp bs i) ! l))"
     using assms *(1) length_nth_bin_\<pi>_it' less_le_trans by blast
-  ultimately show "x \<in> set_bin (bins (\<pi>_it' k bs i) ! l)"
+  ultimately show "x \<in> set_bin (bins (\<pi>_it' k inp bs i) ! l)"
     by simp
 qed
 
 lemma set_bin_\<pi>_it'_eq:
-  "l < k \<Longrightarrow> set_bin (bins (\<pi>_it' k bs i) ! l) = set_bin (bins bs ! l)"
-  by (induction k bs i rule: \<pi>_it'_induct) (auto simp: app_bins_def nth_app_bins)
+  "l < k \<Longrightarrow> set_bin (bins (\<pi>_it' k inp bs i) ! l) = set_bin (bins bs ! l)"
+  by (induction k inp bs i rule: \<pi>_it'_induct) (auto simp: app_bins_def nth_app_bins)
 
 lemma set_bins_upto_k0_\<pi>_it'_eq:
-  "k < length (bins bs) \<Longrightarrow> set_bins_upto (\<pi>_it k bs) k 0 = set_bins_upto bs k 0"
+  "k < length (bins bs) \<Longrightarrow> set_bins_upto (\<pi>_it k inp bs) k 0 = set_bins_upto bs k 0"
   unfolding set_bins_upto_def set_bin_upto_def \<pi>_it_def using set_bin_\<pi>_it'_eq by auto
 
 subsection \<open>Wellformed Bins\<close>
@@ -378,7 +378,7 @@ lemma wf_bins_app_bins:
   by (cases "k < length (bins bs)") (auto simp: nth_list_update, blast+)
 
 lemma wf_bins_Init_it:
-  "wf_bins \<RR> inp Init_it"
+  "wf_bins \<RR> inp (Init_it inp)"
 proof -
   let ?rs = "filter (\<lambda>r. rule_head r = \<SS>) \<RR>"
   let ?b0 = "Bin (map (\<lambda>r. init_item r 0) ?rs)"
@@ -392,7 +392,7 @@ proof -
 qed
 
 lemma distinct_Scan_it:
-  "distinct (Scan_it k a x)"
+  "distinct (Scan_it k inp a x)"
   unfolding Scan_it_def by simp
 
 lemma distinct_Predict_it:
@@ -414,7 +414,7 @@ lemma wf_bins_Scan_it':
 lemma wf_bins_Scan_it:
   assumes "wf_bins \<RR> inp bs" "k < length (bins bs)" "x \<in> set_bin (bins bs ! k)"
   assumes "k \<le> length inp" "next_symbol x \<noteq> None"
-  shows "\<forall>y \<in> set (Scan_it k a x). wf_item \<RR> inp y \<and> item_end y = (k+1)" 
+  shows "\<forall>y \<in> set (Scan_it k inp a x). wf_item \<RR> inp y \<and> item_end y = (k+1)" 
   using wf_bins_Scan_it'[OF assms(1-3) _ assms(5)] 
   by (metis List.list.set(1,2) Scan_it_def empty_iff insert_iff)
 
@@ -432,20 +432,21 @@ lemma wf_bins_Complete_it:
   by (auto, metis le_less_trans, metis le_less_trans le_trans)
 
 lemma wf_bins_\<pi>_it':
-  "wf_bins \<RR> inp bs \<Longrightarrow> k < length (bins bs) \<Longrightarrow> k \<le> length inp \<Longrightarrow> wf_bins \<RR> inp (\<pi>_it' k bs i)"
-proof (induction k bs i arbitrary: I rule: \<pi>_it'_induct)
-  case (Complete k bs i x)
+  "wf_bins \<RR> inp bs \<Longrightarrow> k < length (bins bs) \<Longrightarrow> k \<le> length inp \<Longrightarrow> wf_bins \<RR> inp (\<pi>_it' k inp bs i)"
+proof (induction k inp bs i rule: \<pi>_it'_induct)
+  case (Complete k inp bs i x)
   let ?bs' = "app_bins bs k (Complete_it k x bs)"
   have "x \<in> set_bin (bins bs ! k)"
     using Complete.hyps(1,2) by force
   hence "wf_bins \<RR> inp ?bs'"
     using wf_bins_app_bins Complete.hyps(2) Complete.prems(1,2) wf_bins_Complete_it 
-      distinct_Complete_it wf_bins_kth_bin wf_item_def by (metis nat_less_le order_less_le_trans)
+      distinct_Complete_it wf_bins_kth_bin wf_item_def
+    by (smt (verit, ccfv_SIG) Suc_le_eq less_Suc_eq_le order_less_le_trans)
   thus ?case
     using Complete_\<pi>_mono \<pi>_mono \<pi>_sub_mono \<pi>_idem Complete.IH Complete.hyps Complete.prems(2,3) by fastforce
 next
-  case (Scan k bs i x a)
-  let ?bs' = "app_bins bs (k+1) (Scan_it k a x)"
+  case (Scan k inp bs i x a)
+  let ?bs' = "app_bins bs (k+1) (Scan_it k inp a x)"
   have "x \<in> set_bin (bins bs ! k)"
     using Scan.hyps(1,2) by force
   hence "wf_bins \<RR> inp ?bs'"
@@ -454,7 +455,7 @@ next
     using Scan_\<pi>_mono \<pi>_mono \<pi>_sub_mono \<pi>_idem
     by (metis length_bins_app_bins \<pi>_it'_simps(3) Scan.IH Scan.hyps Scan.prems(2,3))
 next
-  case (Predict k bs i x a)
+  case (Predict k inp bs i x a)
   let ?bs' = "app_bins bs k (Predict_it k a)"
   have "x \<in> set_bin (bins bs ! k)"
     using Predict.hyps(1,2) by force
@@ -467,21 +468,21 @@ next
 qed auto
 
 lemma wf_bins_\<pi>_it:
-  "wf_bins \<RR> inp bs \<Longrightarrow> k < length (bins bs) \<Longrightarrow> k \<le> length inp \<Longrightarrow> wf_bins \<RR> inp (\<pi>_it k bs)"
+  "wf_bins \<RR> inp bs \<Longrightarrow> k < length (bins bs) \<Longrightarrow> k \<le> length inp \<Longrightarrow> wf_bins \<RR> inp (\<pi>_it k inp bs)"
   using \<pi>_it_def wf_bins_\<pi>_it' by presburger
 
 lemma wf_bins_\<I>_it:
-  "k \<le> length inp \<Longrightarrow> wf_bins \<RR> inp (\<I>_it k)"
+  "k \<le> length inp \<Longrightarrow> wf_bins \<RR> inp (\<I>_it k inp)"
   by (induction k) (auto simp: wf_bins_Init_it wf_bins_\<pi>_it)
 
 lemma wf_bins_\<II>_it:
-  "wf_bins \<RR> inp \<II>_it"
+  "wf_bins \<RR> inp (\<II>_it inp)"
   unfolding \<II>_it_def using wf_bins_\<I>_it length_bins_Init_it by auto
 
 subsection \<open>List to Set\<close>
 
 lemma Init_it_eq_Init:
-  "set_bins Init_it = Init"
+  "set_bins (Init_it inp) = Init"
 proof -
   let ?rs = "filter (\<lambda>r. rule_head r = \<SS>) \<RR>"
   let ?b0 = "map (\<lambda>r. init_item r 0) ?rs"
@@ -489,7 +490,7 @@ proof -
   have "set_bins ?bs = {}"
     unfolding set_bins_def set_bins_upto_def set_bin_def set_bin_upto_def
     by (auto simp del: replicate_Suc)
-  hence "set_bins Init_it = set ?b0"
+  hence "set_bins (Init_it inp) = set ?b0"
     by (auto simp: Init_it_def set_bins_app_bins)
   thus ?thesis
     unfolding Init_def rule_head_def using valid_rules by auto
@@ -498,20 +499,20 @@ qed
 lemma Scan_it_sub_Scan:
   assumes "wf_bins \<RR> inp bs" "set_bins bs \<subseteq> I" "x \<in> set_bin (bins bs ! k)" "k < length (bins bs)"
   assumes "next_symbol x = Some a"
-  shows "set (Scan_it k a x) \<subseteq> Scan k I"
+  shows "set (Scan_it k inp a x) \<subseteq> Scan k inp I"
 proof standard
   fix y
-  assume *: "y \<in> set (Scan_it k a x)"
+  assume *: "y \<in> set (Scan_it k inp a x)"
   have "x \<in> bin I k"
     using kth_bin_in_bins assms(1-4) set_bin_def wf_bin_def wf_bins_def bin_def by blast
   {
     assume #: "k < length inp" "inp!k = a"
     hence "y = inc_item x (k+1)"
       using * unfolding Scan_it_def by simp
-    hence "y \<in> Scan k I"
+    hence "y \<in> Scan k inp I"
       using \<open>x \<in> bin I k\<close> # assms(5) unfolding Scan_def by blast
   }
-  thus "y \<in> Scan k I"
+  thus "y \<in> Scan k inp I"
     using * unfolding Scan_it_def by fastforce
 qed
 
@@ -559,14 +560,14 @@ qed
 
 lemma \<pi>_it'_sub_\<pi>:
   assumes "wf_bins \<RR> inp bs" "set_bins bs \<subseteq> I" "length (bins bs) = length inp + 1" "k < length (bins bs)"
-  shows "set_bins (\<pi>_it' k bs i) \<subseteq> \<pi> k I"
+  shows "set_bins (\<pi>_it' k inp bs i) \<subseteq> \<pi> k inp I"
   using assms
-proof (induction k bs i arbitrary: I rule: \<pi>_it'_induct)
-  case (Base k bs i)
+proof (induction k inp bs i arbitrary: I rule: \<pi>_it'_induct)
+  case (Base k inp bs i)
   thus ?case
-    using \<pi>_mono by auto
+    using \<pi>_mono by fastforce
 next
-  case (Complete k bs i x)
+  case (Complete k inp bs i x)
   let ?bs' = "app_bins bs k (Complete_it k x bs)"
   have 0: "x \<in> set_bin (bins bs ! k)"
     using Complete.hyps(1,2) by force
@@ -574,31 +575,32 @@ next
     using 0 Complete_it_sub_Complete Complete.hyps(3) Complete.prems(1,2,4) set_bins_app_bins Un_mono by metis
   moreover have "wf_bins \<RR> inp ?bs'"
     using 0 wf_bins_app_bins Complete.hyps(2) Complete.prems(1,4) wf_bins_Complete_it 
-      distinct_Complete_it wf_bins_kth_bin wf_item_def by (metis add_lessD1 le_Suc_ex)
-  ultimately have "set_bins (\<pi>_it' k bs i) \<subseteq> \<pi> k (I \<union> Complete k I)"
+      distinct_Complete_it wf_bins_kth_bin wf_item_def
+    by (smt (verit, del_insts) le_eq_less_or_eq Complete.hyps(1) order_trans)
+  ultimately have "set_bins (\<pi>_it' k inp bs i) \<subseteq> \<pi> k inp (I \<union> Complete k I)"
     using Complete.IH Complete.hyps Complete.prems(3,4) by simp
   thus ?case
     using Complete_\<pi>_mono \<pi>_mono \<pi>_sub_mono \<pi>_idem by (metis le_supI order_trans)
 next
-  case (Scan k bs i x a)
-  let ?bs' = "app_bins bs (k+1) (Scan_it k a x)"
+  case (Scan k inp bs i x a)
+  let ?bs' = "app_bins bs (k+1) (Scan_it k inp a x)"
   have 0: "x \<in> set_bin (bins bs ! k)"
     using Scan.hyps(1,2) by force
-  have "set_bins ?bs' \<subseteq> I \<union> Scan k I"
+  have "set_bins ?bs' \<subseteq> I \<union> Scan k inp I"
     using 0 Scan_it_sub_Scan[OF Scan.prems(1,2) 0 Scan.prems(4) Scan.hyps(3)]
           Scan.hyps(5) Scan.prems(2,3) by (auto simp: set_bins_app_bins)
   moreover have "wf_bins \<RR> inp ?bs'"
     using 0 wf_bins_Scan_it wf_bins_app_bins Scan.hyps(3,5) Scan.prems(1,4) distinct_Scan_it by force
-  ultimately have "set_bins (\<pi>_it' k bs i) \<subseteq> \<pi> k (I \<union> Scan k I)"
+  ultimately have "set_bins (\<pi>_it' k inp bs i) \<subseteq> \<pi> k inp (I \<union> Scan k inp I)"
     using Scan.IH Scan.hyps Scan.prems(3,4) by simp
   thus ?case
     using Scan_\<pi>_mono \<pi>_mono \<pi>_sub_mono \<pi>_idem by (metis le_supI order_trans)
 next
-  case (Pass k bs i x a)
+  case (Pass k inp bs i x a)
   thus ?case
     using \<pi>_it'_simps(4) by simp
 next
-  case (Predict k bs i x a)
+  case (Predict k inp bs i x a)
   let ?bs' = "app_bins bs k (Predict_it k a)"
   have 0: "x \<in> set_bin (bins bs ! k)"
     using Predict.hyps(1,2) by force
@@ -607,7 +609,7 @@ next
   moreover have "wf_bins \<RR> inp ?bs'"
     using Suc_eq_plus1 Suc_le_eq Suc_le_mono Predict.prems(1,3,4) wf_bins_Predict_it
       wf_bins_app_bins distinct_Predict_it by presburger
-  ultimately have "set_bins (\<pi>_it' k bs i)  \<subseteq> \<pi> k (I \<union> Predict k I)"
+  ultimately have "set_bins (\<pi>_it' k inp bs i)  \<subseteq> \<pi> k inp (I \<union> Predict k I)"
     using Predict.IH Predict.hyps Predict.prems(3,4) by simp
   thus ?case
     using Predict_\<pi>_mono \<pi>_mono \<pi>_sub_mono \<pi>_idem by (metis le_supI order_trans)
@@ -615,82 +617,82 @@ qed
 
 lemma \<pi>_it_sub_\<pi>:
   assumes "wf_bins \<RR> inp bs" "set_bins bs \<subseteq> I" "length (bins bs) = length inp + 1" "k < length (bins bs)"
-  shows "set_bins (\<pi>_it k bs) \<subseteq> \<pi> k I"
+  shows "set_bins (\<pi>_it k inp bs) \<subseteq> \<pi> k inp I"
   using assms \<pi>_it'_sub_\<pi> \<pi>_it_def by metis
 
 lemma \<I>_it_sub_\<I>:
-  "k < length (bins Init_it) \<Longrightarrow> set_bins (\<I>_it k) \<subseteq> \<I> k"
+  "k < length (bins (Init_it inp)) \<Longrightarrow> set_bins (\<I>_it k inp) \<subseteq> \<I> k inp"
   by (induction k) (auto simp: Init_it_eq_Init \<pi>_it_sub_\<pi> wf_bins_Init_it wf_bins_\<I>_it)
 
 lemma \<II>_it_sub_\<II>:
-  "set_bins \<II>_it \<subseteq> \<II>"
+  "set_bins (\<II>_it inp) \<subseteq> \<II> inp"
   using \<I>_it_sub_\<I> \<II>_def \<II>_it_def by auto
 
 subsection \<open>Soundness\<close>
 
 lemma sound_Scan_it:
   assumes "wf_bins \<RR> inp bs" "set_bins bs \<subseteq> I" "x \<in> set_bin (bins bs ! k)" "k < length (bins bs)"
-  assumes "next_symbol x = Some a" "wf_items \<RR> inp I" "sound_items I"
-  shows "sound_items (set (Scan_it k a x))"
+  assumes "next_symbol x = Some a" "wf_items \<RR> inp I" "sound_items inp I"
+  shows "sound_items inp (set (Scan_it k inp a x))"
   using sound_Scan Scan_it_sub_Scan assms by (meson sound_items_def subsetD)
 
 lemma sound_Predict_it:
   assumes "wf_bins \<RR> inp bs" "set_bins bs \<subseteq> I" "x \<in> set_bin (bins bs ! k)" "k < length (bins bs)"
-  assumes "next_symbol x = Some X" "sound_items I"
-  shows "sound_items (set (Predict_it k X))"
+  assumes "next_symbol x = Some X" "sound_items inp I"
+  shows "sound_items inp (set (Predict_it k X))"
   using sound_Predict Predict_it_sub_Predict sound_items_def assms by (meson subsetD)
 
 lemma sound_Complete_it:
   assumes "wf_bins \<RR> inp bs" "set_bins bs \<subseteq> I" "y \<in> set_bin (bins bs ! k)" "k < length (bins bs)"
-  assumes "next_symbol y = None" "wf_items \<RR> inp I" "sound_items I"
-  shows "sound_items (set (Complete_it k y bs))"
+  assumes "next_symbol y = None" "wf_items \<RR> inp I" "sound_items inp I"
+  shows "sound_items inp (set (Complete_it k y bs))"
   using sound_Complete Complete_it_sub_Complete sound_items_def assms by (meson subsetD)
 
 lemma sound_\<pi>_it':
   assumes "wf_bins \<RR> inp bs" "k < length (bins bs)" "length (bins bs) = length inp + 1"
-  assumes "sound_items (set_bins bs)"
-  shows "sound_items (set_bins (\<pi>_it' k bs i))"
+  assumes "sound_items inp (set_bins bs)"
+  shows "sound_items inp (set_bins (\<pi>_it' k inp bs i))"
   using assms
-proof (induction k bs i rule: \<pi>_it'_induct)
-  case (Complete k bs i x)
+proof (induction k inp bs i rule: \<pi>_it'_induct)
+  case (Complete k inp bs i x)
   let ?bs' = "app_bins bs k (Complete_it k x bs)"
   have 0: "x \<in> set_bin (bins bs ! k)"
     using Complete.hyps(1,2) by force
   have "wf_bins \<RR> inp ?bs'"
     using 0 Complete.prems(1,2) wf_bins_Complete_it wf_bins_app_bins distinct_Complete_it
       wf_bins_kth_bin wf_item_def by (smt (verit, ccfv_SIG) le_trans nat_less_le nle_le)
-  moreover have "sound_items (set (Complete_it k x bs))"
+  moreover have "sound_items inp (set (Complete_it k x bs))"
     using 0 sound_Complete_it \<pi>_mono Complete.hyps(3) Complete.prems(1,2,4) set_bins_bin_exists 
             sound_\<pi> wf_\<pi> wf_bins_kth_bin wf_items_def by metis
-  ultimately have "sound_items (set_bins (\<pi>_it' k ?bs' (i + 1)))"
+  ultimately have "sound_items inp (set_bins (\<pi>_it' k inp ?bs' (i + 1)))"
     using Complete.IH Complete.prems(2-4) sound_items_def by (auto simp: set_bins_app_bins)
   thus ?case
     using Complete.hyps by simp
 next
-  case (Scan k bs i x a)
-  let ?bs' = "app_bins bs (k+1) (Scan_it k a x)"
+  case (Scan k inp bs i x a)
+  let ?bs' = "app_bins bs (k+1) (Scan_it k inp a x)"
   have 0: "x \<in> set_bin (bins bs ! k)"
     using Scan.hyps(1,2) by force
   have "wf_bins \<RR> inp ?bs'"
     using 0 Scan.prems(1,2) wf_bins_Scan_it wf_bins_app_bins Scan.hyps(3,5) distinct_Scan_it by simp
-  moreover have "sound_items (set (Scan_it k a x))"
+  moreover have "sound_items inp (set (Scan_it k inp a x))"
     using 0 sound_Scan_it \<pi>_mono Scan.hyps(3) Scan.prems(1,2,4) set_bins_bin_exists 
             sound_\<pi> wf_\<pi> wf_bins_kth_bin wf_items_def by metis
-  ultimately have "sound_items (set_bins (\<pi>_it' k ?bs' (i + 1)))"
+  ultimately have "sound_items inp (set_bins (\<pi>_it' k inp ?bs' (i + 1)))"
     using Scan.IH Scan.prems(2-4) sound_items_def Scan.hyps(5) by (auto simp: set_bins_app_bins)
   thus ?case
     using Scan.hyps by simp
 next
-  case (Predict k bs i x a)
+  case (Predict k inp bs i x a)
   let ?bs' = "app_bins bs k (Predict_it k a)"
   have 0: "x \<in> set_bin (bins bs ! k)"
     using Predict.hyps(1,2) by force
   have "wf_bins \<RR> inp ?bs'"
     using 0 Predict.prems(1-3) wf_bins_Predict_it wf_bins_app_bins distinct_Predict_it by simp
-  moreover have "sound_items (set (Predict_it k a))"
+  moreover have "sound_items inp (set (Predict_it k a))"
     using 0 sound_Predict_it \<pi>_mono Predict.hyps(3) Predict.prems(1,2,4) set_bins_bin_exists 
             sound_\<pi> wf_\<pi> wf_bins_kth_bin wf_items_def by metis
-  ultimately have "sound_items (set_bins (\<pi>_it' k ?bs' (i + 1)))"
+  ultimately have "sound_items inp (set_bins (\<pi>_it' k inp ?bs' (i + 1)))"
     using Predict.IH Predict.prems(2-4) sound_items_def by (auto simp: set_bins_app_bins)
   thus ?case
     using Predict.hyps by simp
@@ -698,8 +700,8 @@ qed simp_all
 
 lemma sound_\<pi>_it:
   assumes "wf_bins \<RR> inp bs" "k < length (bins bs)" "length (bins bs) = length inp + 1"
-  assumes "sound_items (set_bins bs)"
-  shows "sound_items (set_bins (\<pi>_it k bs))"
+  assumes "sound_items inp (set_bins bs)"
+  shows "sound_items inp (set_bins (\<pi>_it k inp bs))"
   using sound_\<pi>_it' assms \<pi>_it_def by simp
 
 subsection \<open>Set to List\<close>
@@ -711,7 +713,7 @@ lemma bin_set_bins_upto_set_bins_eq:
   by (auto simp: nth_list_update set_bin_upto_eq_set_bin wf_bins_kth_bin, metis less_trans, blast)
 
 lemma impossible_complete_item:
-  assumes "wf_item \<RR> inp x" "sound_item x" "is_complete x"  "item_origin x = k" "item_end x = k"
+  assumes "wf_item \<RR> inp x" "sound_item inp x" "is_complete x"  "item_origin x = k" "item_end x = k"
   shows False
 proof -
   have "derives [item_rule_head x] []"
@@ -751,7 +753,7 @@ proof (rule ccontr)
 qed
 
 lemma Complete_Un_eq_nonterminal:
-  assumes "next_symbol z = Some a" "is_nonterminal a" "sound_items I" "item_end z = k" "wf_items \<RR> inp I" "wf_item \<RR> inp z"
+  assumes "next_symbol z = Some a" "is_nonterminal a" "sound_items inp I" "item_end z = k" "wf_items \<RR> inp I" "wf_item \<RR> inp z"
   shows "Complete k (I \<union> {z}) = Complete k I"
 proof (rule ccontr)
   assume "Complete k (I \<union> {z}) \<noteq> Complete k I"
@@ -771,7 +773,7 @@ proof (rule ccontr)
       using *(4) A assms(4) by (auto simp: bin_def)
     moreover have "item_end y = k"
       using *(5) bin_def by blast
-    moreover have "sound_item y"
+    moreover have "sound_item inp y"
       using *(5,6) assms(1,3) by (auto simp: bin_def next_symbol_def sound_items_def)
     moreover have "wf_item \<RR> inp y"
       using *(5) assms(5,6) wf_items_def by (auto simp: bin_def)
@@ -865,40 +867,40 @@ qed
 
 lemma \<pi>_it'_mono:
   assumes "k < length (bins bs)" "length (bins bs) = length inp + 1"
-  shows "set_bins bs \<subseteq> set_bins (\<pi>_it' k bs i)"
-  using assms by (induction k bs i rule: \<pi>_it'_induct) (auto simp: set_bins_app_bins)
+  shows "set_bins bs \<subseteq> set_bins (\<pi>_it' k inp bs i)"
+  using assms by (induction k inp bs i rule: \<pi>_it'_induct) (auto simp: set_bins_app_bins)
 
 lemma \<pi>_step_sub_\<pi>_it':
   assumes "wf_bins \<RR> inp bs" "k < length (bins bs)" "length (bins bs) = length inp + 1"
-  assumes "\<pi>_step k (set_bins_upto bs k i) \<subseteq> set_bins bs"
-  assumes "sound_items (set_bins bs)" "set inp \<subseteq> set \<TT>"
-  shows "\<pi>_step k (set_bins bs) \<subseteq> set_bins (\<pi>_it' k bs i)"
+  assumes "\<pi>_step k inp (set_bins_upto bs k i) \<subseteq> set_bins bs"
+  assumes "sound_items inp (set_bins bs)" "set inp \<subseteq> set \<TT>"
+  shows "\<pi>_step k inp (set_bins bs) \<subseteq> set_bins (\<pi>_it' k inp bs i)"
   using assms
-proof (induction k bs i rule: \<pi>_it'_induct)
-  case (Base k bs i)
+proof (induction k inp bs i rule: \<pi>_it'_induct)
+  case (Base k inp bs i)
   have "bin (set_bins bs) k = bin (set_bins_upto bs k i) k"
     using Base.hyps Base.prems(1,2) bin_set_bins_upto_set_bins_eq by simp
   thus ?case
     using Scan_bin_absorb Predict_bin_absorb Complete_set_bins_upto_eq_set_bins 
       Base.hyps Base.prems(1,2,4) \<pi>_step_def by (auto; metis in_mono)
 next
-  case (Complete k bs i x)
+  case (Complete k inp bs i x)
   let ?bs' = "app_bins bs k (Complete_it k x bs)"
   have x: "x \<in> set_bin (bins bs ! k)"
     using Complete.hyps(1,2) by auto
   have wf: "wf_bins \<RR> inp ?bs'"
     using Complete.hyps Complete.prems(1,2) wf_bins_Complete_it wf_bins_app_bins set_bin_def
       distinct_Complete_it wf_bins_kth_bin wf_item_def x by (smt (verit, best) le_trans nat_less_le nle_le)
-  have sound: "sound_items (set_bins ?bs')"
+  have sound: "sound_items inp (set_bins ?bs')"
     using sound_Complete_it[OF _ _ _ Complete.prems(2) Complete.hyps(3)] wf_bins_impl_wf_items 
           Complete.hyps(1,2) sound_items_def Complete.prems(1,2,5) by (auto simp: set_bins_app_bins)
-  have "Scan k (set_bins_upto ?bs' k (i + 1)) \<subseteq> set_bins ?bs'"
+  have "Scan k inp (set_bins_upto ?bs' k (i + 1)) \<subseteq> set_bins ?bs'"
   proof -
-    have "Scan k (set_bins_upto ?bs' k (i + 1)) = Scan k (set_bins_upto ?bs' k i \<union> {items (bins ?bs' ! k) ! i})"
+    have "Scan k inp (set_bins_upto ?bs' k (i + 1)) = Scan k inp (set_bins_upto ?bs' k i \<union> {items (bins ?bs' ! k) ! i})"
       using Complete.hyps(1) set_bins_upto_Suc_Un length_nth_bin_app_bins by (metis less_le_trans not_le_imp_less)
-    also have "... = Scan k (set_bins_upto bs k i \<union> {x})"
+    also have "... = Scan k inp (set_bins_upto bs k i \<union> {x})"
       using Complete.hyps(1,2) Complete.prems(2) kth_app_bins set_bins_upto_kth_nth_id by (metis leI less_not_refl)
-    also have "... \<subseteq> set_bins bs \<union> Scan k {x}"
+    also have "... \<subseteq> set_bins bs \<union> Scan k inp {x}"
       using Complete.prems(3,4) Scan_Un Scan_\<pi>_step_mono by fastforce
     also have "... = set_bins bs"
       using Complete.hyps(3) Complete.prems(1,2) kth_bin_in_bins wf_bins_kth_bin Scan_def by (auto simp: bin_def)
@@ -930,50 +932,50 @@ next
     finally show ?thesis
       using Complete.prems(2) set_bins_app_bins by blast
   qed
-  ultimately have "\<pi>_step k (set_bins ?bs') \<subseteq> set_bins (\<pi>_it' k ?bs' (i+1))"
+  ultimately have "\<pi>_step k inp (set_bins ?bs') \<subseteq> set_bins (\<pi>_it' k inp ?bs' (i+1))"
     using Complete.IH Complete.prems(2,3,6) sound wf \<pi>_step_def set_bins_upto_sub_set_bins
     by (metis (no_types, lifting) Un_assoc length_bins_app_bins subset_Un_eq)
   thus ?case
     using \<pi>_it'_simps(2) \<pi>_step_sub_mono Complete.hyps local.Complete.prems(2) set_bins_app_bins
     by (smt (verit, del_insts) Orderings.preorder_class.dual_order.trans Un_upper1)
 next
-  case (Scan k bs i x a)
-  let ?bs' = "app_bins bs (k+1) (Scan_it k a x)"
+  case (Scan k inp bs i x a)
+  let ?bs' = "app_bins bs (k+1) (Scan_it k inp a x)"
   have x: "x \<in> set_bin (bins bs ! k)"
     using Scan.hyps(1,2) by auto
   have wf: "wf_bins \<RR> inp ?bs'"
     using Scan.prems(1,2) Scan.hyps wf_bins_app_bins wf_bins_Scan_it x distinct_Scan_it by (metis Option.option.discI nat_less_le)
-  have sound: "sound_items (set_bins ?bs')"
+  have sound: "sound_items inp (set_bins ?bs')"
     using sound_Scan_it[OF Scan.prems(1) _ x Scan.prems(2)] Scan.hyps(3,5) Scan.prems(1,3,5) 
           sound_items_def wf_bins_impl_wf_items by (auto simp: set_bins_app_bins, blast)
-  have "Scan k (set_bins_upto ?bs' k (i + 1)) \<subseteq> set_bins ?bs'"
+  have "Scan k inp (set_bins_upto ?bs' k (i + 1)) \<subseteq> set_bins ?bs'"
   proof -
-    have "Scan k (set_bins_upto ?bs' k (i + 1)) = Scan k (set_bins_upto ?bs' k i \<union> {items (bins ?bs' ! k) ! i})"
+    have "Scan k inp (set_bins_upto ?bs' k (i + 1)) = Scan k inp (set_bins_upto ?bs' k i \<union> {items (bins ?bs' ! k) ! i})"
       using set_bins_upto_Suc_Un Scan.hyps(1) nth_app_bins
       by (metis Groups.monoid_add_class.add.right_neutral One_nat_def add_Suc_right lessI less_not_refl not_le_imp_less)
-    also have "... = Scan k (set_bins_upto bs k i \<union> {x})"
+    also have "... = Scan k inp (set_bins_upto bs k i \<union> {x})"
       using Scan.hyps(1,2,5) Scan.prems(3) nth_app_bins set_bins_upto_kth_nth_id
       by (metis (no_types, lifting) Suc_eq_plus1 Suc_less_eq lessI linorder_not_less nat_less_le)
-    also have "... \<subseteq> set_bins bs \<union> Scan k {x}"
+    also have "... \<subseteq> set_bins bs \<union> Scan k inp {x}"
       using Scan.prems(3,4) Scan_Un Scan_\<pi>_step_mono by fastforce
-    finally have *: "Scan k (set_bins_upto ?bs' k (i + 1)) \<subseteq> set_bins bs \<union> Scan k {x}" .
+    finally have *: "Scan k inp (set_bins_upto ?bs' k (i + 1)) \<subseteq> set_bins bs \<union> Scan k inp {x}" .
     show ?thesis
     proof cases
       assume a1: "inp!k = a"
-      hence "Scan k {x} = {inc_item x (k+1)}"
+      hence "Scan k inp {x} = {inc_item x (k+1)}"
         using Scan_def Scan.hyps(1-3,5) wf_bins_kth_bin bin_def Scan.prems(1,2) by (auto simp: bin_def)
-      hence "Scan k (set_bins_upto ?bs' k (i + 1)) \<subseteq> set_bins bs \<union> {inc_item x (k+1)}"
+      hence "Scan k inp (set_bins_upto ?bs' k (i + 1)) \<subseteq> set_bins bs \<union> {inc_item x (k+1)}"
         using * by blast
-      also have "... = set_bins bs \<union> set (Scan_it k a x)"
+      also have "... = set_bins bs \<union> set (Scan_it k inp a x)"
         using Scan_it_def a1 Scan.hyps(5) by force
       also have "... = set_bins ?bs'"
         using Scan.hyps(5) Scan.prems(3) by (auto simp: set_bins_app_bins)
       finally show ?thesis .
     next
       assume a1: "\<not> inp!k = a"
-      hence "Scan k {x} = {}"
+      hence "Scan k inp {x} = {}"
         using Scan_def bin_def Scan.hyps(3) by (auto simp: bin_def)
-      hence "Scan k (set_bins_upto ?bs' k (i + 1)) \<subseteq> set_bins bs"
+      hence "Scan k inp (set_bins_upto ?bs' k (i + 1)) \<subseteq> set_bins bs"
         using * by blast
       also have "... \<subseteq> set_bins ?bs'"
         using Scan.hyps(5) Scan.prems(3) by (auto simp: set_bins_app_bins)
@@ -1008,15 +1010,15 @@ next
     finally show ?thesis
       using Scan.hyps(5) Scan.prems(3,4) Complete_\<pi>_step_mono by (auto simp: set_bins_app_bins, blast)
   qed
-  ultimately have "\<pi>_step k (set_bins ?bs') \<subseteq> set_bins (\<pi>_it' k ?bs' (i+1))"
+  ultimately have "\<pi>_step k inp (set_bins ?bs') \<subseteq> set_bins (\<pi>_it' k inp ?bs' (i+1))"
     using Scan.IH Scan.prems(2,3,6) sound wf \<pi>_step_def set_bins_upto_sub_set_bins by (metis Un_subset_iff length_bins_app_bins)
   thus ?case
     using \<pi>_step_sub_mono \<pi>_it'_simps(3) Scan.hyps Scan.prems(2,3) by (auto simp: set_bins_app_bins, blast)
 next
-  case (Pass k bs i x a)
+  case (Pass k inp bs i x a)
   have x: "x \<in> set_bin (bins bs ! k)"
     using Pass.hyps(1,2) by auto
-  have "Scan k (set_bins_upto bs k (i + 1)) \<subseteq> set_bins bs"
+  have "Scan k inp (set_bins_upto bs k (i + 1)) \<subseteq> set_bins bs"
     using Scan_def Pass.hyps(5) by blast
   moreover have "Predict k (set_bins_upto bs k (i + 1)) \<subseteq> set_bins bs"
   proof -
@@ -1041,12 +1043,12 @@ next
     finally show ?thesis
       using Pass.prems(4) Complete_\<pi>_step_mono by blast
   qed
-  ultimately have "\<pi>_step k (set_bins bs) \<subseteq> set_bins (\<pi>_it' k bs (i+1))"
+  ultimately have "\<pi>_step k inp (set_bins bs) \<subseteq> set_bins (\<pi>_it' k inp bs (i+1))"
     using Pass.IH Pass.prems(1-3,5,6) \<pi>_step_def set_bins_upto_sub_set_bins by (metis Un_subset_iff)
   thus ?case
     using set_bins_app_bins Pass.hyps Pass.prems by simp
 next
-  case (Predict k bs i x a)
+  case (Predict k inp bs i x a)
   let ?bs' = "app_bins bs k (Predict_it k a)"
   have "k \<ge> length inp \<or> \<not> inp!k = a"
     using Predict.hyps(4) is_terminal_def Predict.prems(6) by force
@@ -1056,17 +1058,17 @@ next
     using length_nth_bin_app_bins Predict.hyps(1) by (metis leI order_less_le_trans)
   have wf: "wf_bins \<RR> inp ?bs'"
     using Predict.prems(1-3) wf_bins_Predict_it wf_bins_app_bins distinct_Predict_it by force
-  have sound: "sound_items (set_bins ?bs')" 
+  have sound: "sound_items inp (set_bins ?bs')" 
     using sound_Predict_it[OF _ _ x] Predict.hyps(3) Predict.prems(1,2,5) sound_items_def by (auto simp: set_bins_app_bins)
   have nonterm: "is_nonterminal a"
     using is_symbol_distinct Predict.hyps(3,4) Predict.prems(1,2) wf_bins_kth_bin x by blast
-  have "Scan k (set_bins_upto ?bs' k (i + 1)) \<subseteq> set_bins ?bs'"
+  have "Scan k inp (set_bins_upto ?bs' k (i + 1)) \<subseteq> set_bins ?bs'"
   proof -
-    have "Scan k (set_bins_upto ?bs' k (i + 1)) = Scan k (set_bins_upto ?bs' k i \<union> {items (bins ?bs' ! k) ! i})"
+    have "Scan k inp (set_bins_upto ?bs' k (i + 1)) = Scan k inp (set_bins_upto ?bs' k i \<union> {items (bins ?bs' ! k) ! i})"
       using Predict.hyps(1) set_bins_upto_Suc_Un length_nth_bin_app_bins by (metis less_le_trans not_le_imp_less)
-    also have "... = Scan k (set_bins_upto bs k i \<union> {x})"
+    also have "... = Scan k inp (set_bins_upto bs k i \<union> {x})"
       using Predict.hyps(1,2) Predict.prems(2) kth_app_bins set_bins_upto_kth_nth_id by (metis less_not_refl not_le_imp_less)
-    also have "... \<subseteq> set_bins bs \<union> Scan k {x}"
+    also have "... \<subseteq> set_bins bs \<union> Scan k inp {x}"
       using Predict.prems(3,4) Scan_Un Scan_\<pi>_step_mono by fastforce
     also have "... = set_bins bs"
       using Predict.hyps(3) \<open>length inp \<le> k \<or> inp ! k \<noteq> a\<close> Scan_def by (auto simp: bin_def)
@@ -1094,11 +1096,12 @@ next
       using kth_app_bins Predict.hyps(1,2) Predict.prems(2) set_bins_upto_kth_nth_id by (metis leI nle_le)
     also have "... = Complete k (set_bins_upto bs k i)"
       using Complete_Un_eq_nonterminal nonterm Predict.hyps(3) Predict.prems(1,2,5) set_bins_upto_sub_set_bins 
-            sound_items_def subset_eq wf_bins_kth_bin x wf_bins_impl_wf_items wf_items_def by metis
+            sound_items_def subset_eq wf_bins_kth_bin x wf_bins_impl_wf_items wf_items_def
+      by (smt (verit, ccfv_SIG))
     finally show ?thesis
       using set_bins_app_bins Predict.prems(2,4) Complete_\<pi>_step_mono by fastforce
   qed
-  ultimately have "\<pi>_step k (set_bins ?bs') \<subseteq> set_bins (\<pi>_it' k ?bs' (i+1))"
+  ultimately have "\<pi>_step k inp (set_bins ?bs') \<subseteq> set_bins (\<pi>_it' k inp ?bs' (i+1))"
     using Predict.IH Predict.prems(2,3,6) sound wf \<pi>_step_def set_bins_upto_sub_set_bins 
     by (metis Un_subset_iff length_bins_app_bins)
   thus ?case
@@ -1107,25 +1110,26 @@ qed
 
 lemma \<pi>_step_sub_\<pi>_it:
   assumes "wf_bins \<RR> inp bs" "k < length (bins bs)" "length (bins bs) = length inp + 1"
-  assumes "\<pi>_step k (set_bins_upto bs k 0) \<subseteq> set_bins bs"
-  assumes "sound_items (set_bins bs)" "set inp \<subseteq> set \<TT>"
-  shows "\<pi>_step k (set_bins bs) \<subseteq> set_bins (\<pi>_it k bs)"
+  assumes "\<pi>_step k inp (set_bins_upto bs k 0) \<subseteq> set_bins bs"
+  assumes "sound_items inp (set_bins bs)" "set inp \<subseteq> set \<TT>"
+  shows "\<pi>_step k inp (set_bins bs) \<subseteq> set_bins (\<pi>_it k inp bs)"
   using assms \<pi>_step_sub_\<pi>_it' \<pi>_it_def by metis
 
 lemma \<pi>_it'_idem:
   assumes "wf_bins \<RR> inp bs" "k < length (bins bs)" "length (bins bs) = length inp + 1" "i \<le> j"
-  assumes "sound_items (set_bins bs)"
-  shows "\<pi>_it' k (\<pi>_it' k bs i) j = \<pi>_it' k bs i"
+  assumes "sound_items inp (set_bins bs)"
+  shows "\<pi>_it' k inp (\<pi>_it' k inp bs i) j = \<pi>_it' k inp bs i"
   using assms
-proof (induction k bs i arbitrary: j rule: \<pi>_it'_induct)
-  case (Complete k bs i x)
+proof (induction k inp bs i arbitrary: j rule: \<pi>_it'_induct)
+  case (Complete k inp bs i x)
   let ?bs' = "app_bins bs k (Complete_it k x bs)"
   have x: "x \<in> set_bin (bins bs ! k)"
     using Complete.hyps(1,2) by auto
   have wf: "wf_bins \<RR> inp ?bs'"
     using Complete.hyps Complete.prems(1,2) wf_bins_Complete_it wf_bins_app_bins
-      distinct_Complete_it wf_bins_kth_bin wf_item_def x by (metis linorder_not_less order_less_le_trans)
-  have sound: "sound_items (set_bins ?bs')"
+      distinct_Complete_it wf_bins_kth_bin wf_item_def x
+    by (smt (verit) linorder_not_less order_trans)
+  have sound: "sound_items inp (set_bins ?bs')"
     using sound_Complete_it[OF _ _ _ Complete.prems(2) Complete.hyps(3)] wf_bins_impl_wf_items 
           Complete.hyps(1,2) sound_items_def Complete.prems(1,2,5) by (auto simp: set_bins_app_bins)
   show ?case
@@ -1137,11 +1141,11 @@ proof (induction k bs i arbitrary: j rule: \<pi>_it'_induct)
     assume "\<not> i+1 \<le> j"
     hence "i = j"
       using Complete.prems(4) by simp
-    have "\<pi>_it' k (\<pi>_it' k bs i) j = \<pi>_it' k (\<pi>_it' k ?bs' (i+1)) j"
+    have "\<pi>_it' k inp (\<pi>_it' k inp bs i) j = \<pi>_it' k inp (\<pi>_it' k inp ?bs' (i+1)) j"
       using \<pi>_it'_simps(2) Complete.hyps(1-3) by presburger
-    also have "... = \<pi>_it' k (\<pi>_it' k ?bs' (i+1)) (j+1)"
+    also have "... = \<pi>_it' k inp (\<pi>_it' k inp ?bs' (i+1)) (j+1)"
     proof -
-      let ?bs'' = "\<pi>_it' k ?bs' (i+1)"
+      let ?bs'' = "\<pi>_it' k inp ?bs' (i+1)"
       have "length (items (bins ?bs'' ! k)) \<ge> length (items (bins bs ! k))"
         using length_nth_bin_\<pi>_it' length_nth_bin_app_bins order_trans by blast
       hence 0: "\<not> length (items (bins ?bs'' ! k)) \<le> j"
@@ -1150,7 +1154,7 @@ proof (induction k bs i arbitrary: j rule: \<pi>_it'_induct)
         using \<open>i = j\<close> kth_app_bins Complete.hyps(1,2) by (metis not_le_imp_less)
       hence 1: "x = items (bins ?bs'' ! k) ! j"
         using \<open>i = j\<close> kth_\<pi>_it'_bins length_nth_bin_app_bins Complete.hyps(1) by (metis leI order_trans)
-      have "\<pi>_it' k ?bs'' j = \<pi>_it' k (app_bins ?bs'' k (Complete_it k x ?bs'')) (j+1)"
+      have "\<pi>_it' k inp ?bs'' j = \<pi>_it' k inp (app_bins ?bs'' k (Complete_it k x ?bs'')) (j+1)"
         using \<pi>_it'_simps(2) 0 1 Complete.hyps(1,3) Complete.prems(2)
         by (metis calculation length_bins_\<pi>_it' wf wf_bins_\<pi>_it' wf_bins_kth_bin wf_item_def x)
       moreover have "app_bins ?bs'' k (Complete_it k x ?bs'') = ?bs''"
@@ -1164,7 +1168,7 @@ proof (induction k bs i arbitrary: j rule: \<pi>_it'_induct)
         next
           case False
           hence "item_origin x < k"
-            using x Complete.prems(1,2) wf_bins_kth_bin wf_item_def by force
+            using x Complete.prems(1,2) wf_bins_kth_bin wf_item_def nat_less_le by blast
           hence "set_bin (bins bs ! item_origin x) = set_bin (bins ?bs'' ! item_origin x)"
             using False app_bins_def set_bin_\<pi>_it'_eq by (simp add: nth_app_bins)
           thus ?thesis
@@ -1181,20 +1185,20 @@ proof (induction k bs i arbitrary: j rule: \<pi>_it'_induct)
       ultimately show ?thesis
         by presburger
     qed
-    also have "... = \<pi>_it' k ?bs' (i + 1)"
+    also have "... = \<pi>_it' k inp ?bs' (i + 1)"
       using Complete.IH Complete.prems(1-3) \<open>i = j\<close> Complete.hyps length_bins_app_bins 
             wf_bins_Complete_it wf_bins_app_bins x wf sound by (metis le_refl)
     finally show ?thesis
       using Complete.hyps by simp
   qed
 next
-  case (Scan k bs i x a)
-  let ?bs' = "app_bins bs (k+1) (Scan_it k a x)"
+  case (Scan k inp bs i x a)
+  let ?bs' = "app_bins bs (k+1) (Scan_it k inp a x)"
   have x: "x \<in> set_bin (bins bs ! k)"
     using Scan.hyps(1,2) by auto
   have wf: "wf_bins \<RR> inp ?bs'"
     using Scan.prems(1,2) Scan.hyps wf_bins_app_bins wf_bins_Scan_it x distinct_Scan_it by (metis Option.option.discI nat_less_le)
-  have sound: "sound_items (set_bins ?bs')"
+  have sound: "sound_items inp (set_bins ?bs')"
     using sound_Scan_it[OF Scan.prems(1) _ x Scan.prems(2)] Scan.hyps(3,5) Scan.prems(1,3,5) 
           set_bins_app_bins sound_items_def wf_bins_impl_wf_items
     by (metis Groups.ab_semigroup_add_class.add.commute Orderings.preorder_class.dual_order.refl UnE add_less_cancel_left)
@@ -1207,40 +1211,40 @@ next
     assume "\<not> i+1 \<le> j"
     hence "i = j"
       using Scan.prems(4) by auto
-    have "\<pi>_it' k (\<pi>_it' k bs i) j = \<pi>_it' k (\<pi>_it' k ?bs' (i+1)) j"
+    have "\<pi>_it' k inp (\<pi>_it' k inp bs i) j = \<pi>_it' k inp (\<pi>_it' k inp ?bs' (i+1)) j"
       using Scan.hyps by simp
-    also have "... = \<pi>_it' k (\<pi>_it' k ?bs' (i+1)) (j+1)"
+    also have "... = \<pi>_it' k inp (\<pi>_it' k inp ?bs' (i+1)) (j+1)"
     proof -
-      let ?bs'' = "\<pi>_it' k ?bs' (i+1)"
+      let ?bs'' = "\<pi>_it' k inp ?bs' (i+1)"
       have "length (items (bins ?bs'' ! k)) \<ge> length (items (bins bs ! k))"
         using length_nth_bin_\<pi>_it' length_nth_bin_app_bins order_trans by blast
-      hence "\<pi>_it' k ?bs'' j = \<pi>_it' k (app_bins ?bs'' (k+1) (Scan_it k a x)) (j+1)"
+      hence "\<pi>_it' k inp ?bs'' j = \<pi>_it' k inp (app_bins ?bs'' (k+1) (Scan_it k inp a x)) (j+1)"
         using \<open>i = j\<close> kth_\<pi>_it'_bins nth_app_bin \<pi>_it'_simps(3) Scan.hyps
         by (smt (verit, ccfv_SIG) length_bins_\<pi>_it' less_or_eq_imp_le not_le_imp_less order_trans wf_bins_\<pi>_it')
-      moreover have "app_bins ?bs'' (k+1) (Scan_it k a x) = ?bs''"
+      moreover have "app_bins ?bs'' (k+1) (Scan_it k inp a x) = ?bs''"
       proof -
-        have "set (Scan_it k a x) = set (Scan_it k a x)"
+        have "set (Scan_it k inp a x) = set (Scan_it k inp a x)"
           unfolding Scan_it_def by blast
         also have "... \<subseteq> set_bin (bins ?bs' ! (k+1))"
           using Scan.hyps(5) Scan.prems(3) app_bins_def set_bin_app_bin
           by (metis bins.sel Groups.ab_semigroup_add_class.add.commute Suc_less_eq Un_iff nth_list_update_eq plus_1_eq_Suc subsetI)
         also have "... \<subseteq> set_bin (bins ?bs'' ! (k+1))"
           using Scan.hyps(5) Scan.prems(3) nth_bin_sub_\<pi>_it' by auto
-        ultimately have "set (Scan_it k a x) \<subseteq> set_bin (bins ?bs'' ! (k+1))"
-          using \<open>set (Scan_it k a x) \<subseteq> set_bin (bins (app_bins bs (k + 1) (Scan_it k a x)) ! (k + 1))\<close> by blast
+        ultimately have "set (Scan_it k inp a x) \<subseteq> set_bin (bins ?bs'' ! (k+1))"
+          using \<open>set (Scan_it k inp a x) \<subseteq> set_bin (bins (app_bins bs (k + 1) (Scan_it k inp a x)) ! (k + 1))\<close> by blast
         thus ?thesis
           using app_bins_eq Scan.hyps(5) Scan.prems(3) length_bins_\<pi>_it' by simp
       qed
       ultimately show ?thesis
         by presburger
     qed
-    also have "... = \<pi>_it' k ?bs' (i + 1)"
+    also have "... = \<pi>_it' k inp ?bs' (i + 1)"
       using \<open>i = j\<close> Scan.IH Scan.prems(2,3) sound wf by (metis length_bins_app_bins order_refl)
     finally show ?thesis
       using Scan.hyps by simp
   qed
 next
-  case (Pass k bs i x a)
+  case (Pass k inp bs i x a)
   show ?case
   proof cases
     assume "i+1 \<le> j"
@@ -1252,7 +1256,7 @@ next
       using Pass \<pi>_it'_simps(1,4) kth_\<pi>_it'_bins by (metis Suc_eq_plus1 Suc_leI antisym_conv2 not_le_imp_less)
   qed
 next
-  case (Predict k bs i x a)
+  case (Predict k inp bs i x a)
   let ?bs' = "app_bins bs k (Predict_it k a)"
   have x: "x \<in> set_bin (bins bs ! k)"
     using Predict.hyps(1,2) by auto
@@ -1260,7 +1264,7 @@ next
     using length_nth_bin_app_bins Predict.hyps(1) Orderings.preorder_class.dual_order.strict_trans1 linorder_not_less by blast
   have wf: "wf_bins \<RR> inp ?bs'"
     using Predict.prems(1-3) wf_bins_Predict_it wf_bins_app_bins distinct_Predict_it by force
-  have sound: "sound_items (set_bins ?bs')" 
+  have sound: "sound_items inp (set_bins ?bs')" 
     using sound_Predict_it[OF _ _ x] Predict.hyps(3) Predict.prems(1,2,5) sound_items_def by (auto simp: set_bins_app_bins)
   show ?case
   proof cases
@@ -1271,14 +1275,14 @@ next
     assume "\<not> i+1 \<le> j"
     hence "i = j"
       using Predict.prems(4) by auto
-    have "\<pi>_it' k (\<pi>_it' k bs i) j = \<pi>_it' k (\<pi>_it' k ?bs' (i+1)) j"
+    have "\<pi>_it' k inp (\<pi>_it' k inp bs i) j = \<pi>_it' k inp (\<pi>_it' k inp ?bs' (i+1)) j"
       using Predict.hyps by simp
-    also have "... = \<pi>_it' k (\<pi>_it' k ?bs' (i+1)) (j+1)"
+    also have "... = \<pi>_it' k inp (\<pi>_it' k inp ?bs' (i+1)) (j+1)"
     proof -
-      let ?bs'' = "\<pi>_it' k ?bs' (i+1)"
+      let ?bs'' = "\<pi>_it' k inp ?bs' (i+1)"
       have "length (items (bins ?bs'' ! k)) \<ge> length (items (bins bs ! k))"
         using length_nth_bin_\<pi>_it' length_nth_bin_app_bins order_trans by blast
-      hence "\<pi>_it' k ?bs'' j = \<pi>_it' k (app_bins ?bs'' k (Predict_it k a)) (j+1)"
+      hence "\<pi>_it' k inp ?bs'' j = \<pi>_it' k inp (app_bins ?bs'' k (Predict_it k a)) (j+1)"
         using \<open>i = j\<close> kth_\<pi>_it'_bins nth_app_bin \<pi>_it'_simps(5) Predict.hyps Predict.prems(3) length_bins_\<pi>_it'
           wf_bins_\<pi>_it' by (smt (verit, best) Orderings.preorder_class.dual_order.trans leI wf_bins_kth_bin wf_item_def x)
       moreover have "app_bins ?bs'' k (Predict_it k a) = ?bs''"
@@ -1297,7 +1301,7 @@ next
       ultimately show ?thesis
         by presburger
     qed
-    also have "... = \<pi>_it' k ?bs' (i + 1)"
+    also have "... = \<pi>_it' k inp ?bs' (i + 1)"
       using \<open>i = j\<close> Predict.IH Predict.prems(2,3) sound wf by (metis length_bins_app_bins order_refl)
     finally show ?thesis
       using Predict.hyps by simp
@@ -1305,14 +1309,14 @@ next
 qed simp
 
 lemma \<pi>_it_idem:
-  assumes "wf_bins \<RR> inp bs" "k < length (bins bs)" "length (bins bs) = length inp + 1" "sound_items (set_bins bs)"
-  shows "\<pi>_it k (\<pi>_it k bs) = \<pi>_it k bs"
+  assumes "wf_bins \<RR> inp bs" "k < length (bins bs)" "length (bins bs) = length inp + 1" "sound_items inp (set_bins bs)"
+  shows "\<pi>_it k inp (\<pi>_it k inp bs) = \<pi>_it k inp bs"
   using assms \<pi>_it'_idem \<pi>_it_def le0 by metis
 
 lemma funpower_\<pi>_step_sub_\<pi>_it:
   assumes "wf_bins \<RR> inp bs" "k < length (bins bs)" "length (bins bs) = length inp + 1"
-  assumes "\<pi>_step k (set_bins_upto bs k 0) \<subseteq> set_bins bs" "sound_items (set_bins bs)" "set inp \<subseteq> set \<TT>"
-  shows "funpower (\<pi>_step k) n (set_bins bs) \<subseteq> set_bins (\<pi>_it k bs)"
+  assumes "\<pi>_step k inp (set_bins_upto bs k 0) \<subseteq> set_bins bs" "sound_items inp (set_bins bs)" "set inp \<subseteq> set \<TT>"
+  shows "funpower (\<pi>_step k inp) n (set_bins bs) \<subseteq> set_bins (\<pi>_it k inp bs)"
   using assms
 proof (induction n)
   case 0
@@ -1320,51 +1324,51 @@ proof (induction n)
     using \<pi>_it'_mono \<pi>_it_def by simp
 next
   case (Suc n)
-  have 0: "\<pi>_step k (set_bins_upto (\<pi>_it k bs) k 0) \<subseteq> set_bins (\<pi>_it k bs)"
+  have 0: "\<pi>_step k inp (set_bins_upto (\<pi>_it k inp bs) k 0) \<subseteq> set_bins (\<pi>_it k inp bs)"
     using \<pi>_it'_mono set_bins_upto_k0_\<pi>_it'_eq \<pi>_it_def Suc.prems(2-4) order_trans by metis
-  have "funpower (\<pi>_step k) (Suc n) (set_bins bs) \<subseteq> (\<pi>_step k) (set_bins (\<pi>_it k bs))"
+  have "funpower (\<pi>_step k inp) (Suc n) (set_bins bs) \<subseteq> (\<pi>_step k inp) (set_bins (\<pi>_it k inp bs))"
     using \<pi>_step_sub_mono Suc by auto
-  also have "... \<subseteq> set_bins (\<pi>_it k (\<pi>_it k bs))"
+  also have "... \<subseteq> set_bins (\<pi>_it k inp (\<pi>_it k inp bs))"
     using \<pi>_step_sub_\<pi>_it Suc.prems(1-3,5,6) wf_bins_\<pi>_it sound_\<pi>_it 0 by simp
-  also have "... \<subseteq> set_bins (\<pi>_it k bs)"
+  also have "... \<subseteq> set_bins (\<pi>_it k inp bs)"
     using \<pi>_it_idem Suc.prems by simp
   finally show ?case .
 qed
 
 lemma \<pi>_sub_\<pi>_it:
   assumes "wf_bins \<RR> inp bs" "k < length (bins bs)" "length (bins bs) = length inp + 1"
-  assumes "\<pi>_step k (set_bins_upto bs k 0) \<subseteq> set_bins bs" "sound_items (set_bins bs)" "set inp \<subseteq> set \<TT>"
-  shows "\<pi> k (set_bins bs) \<subseteq> set_bins (\<pi>_it k bs)"
+  assumes "\<pi>_step k inp (set_bins_upto bs k 0) \<subseteq> set_bins bs" "sound_items inp (set_bins bs)" "set inp \<subseteq> set \<TT>"
+  shows "\<pi> k inp (set_bins bs) \<subseteq> set_bins (\<pi>_it k inp bs)"
   using assms funpower_\<pi>_step_sub_\<pi>_it \<pi>_def elem_limit_simp by fastforce
 
 lemma \<I>_sub_\<I>_it:
-  "k < length (bins Init_it) \<Longrightarrow> set inp \<subseteq> set \<TT> \<Longrightarrow> \<I> k \<subseteq> set_bins (\<I>_it k)"
+  "k < length (bins (Init_it inp)) \<Longrightarrow> set inp \<subseteq> set \<TT> \<Longrightarrow> \<I> k inp \<subseteq> set_bins (\<I>_it k inp)"
 proof (induction k)
   case 0
-  hence "\<pi> 0 Init \<subseteq> set_bins (\<pi>_it 0 Init_it)"
+  hence "\<pi> 0 inp Init \<subseteq> set_bins (\<pi>_it 0 inp (Init_it inp))"
     using wf_bins_Init_it \<pi>_sub_\<pi>_it Init_it_eq_Init length_bins_Init_it Init_it_eq_Init 
           sound_Init set_bins_upto_empty \<pi>_step_empty set_bins_upto_sub_set_bins by metis
   thus ?case
     by simp
 next
   case (Suc k)
-  have wf: "wf_bins \<RR> inp (\<I>_it k)"
+  have wf: "wf_bins \<RR> inp (\<I>_it k inp)"
     using length_bins_Init_it Suc.prems wf_bins_\<I>_it by force
-  have sub: "\<pi>_step (Suc k) (set_bins_upto (\<I>_it k) (Suc k) 0) \<subseteq> set_bins (\<I>_it k)"
+  have sub: "\<pi>_step (Suc k) inp (set_bins_upto (\<I>_it k inp) (Suc k) 0) \<subseteq> set_bins (\<I>_it k inp)"
   proof -
-    have "bin (set_bins_upto (\<I>_it k) (Suc k) 0) (Suc k) = {}"
+    have "bin (set_bins_upto (\<I>_it k inp) (Suc k) 0) (Suc k) = {}"
       using kth_bin_set_bins_upto_empty wf Suc.prems by auto
-    hence "\<pi>_step (Suc k) (set_bins_upto (\<I>_it k) (Suc k) 0) = set_bins_upto (\<I>_it k) (Suc k) 0"
+    hence "\<pi>_step (Suc k) inp (set_bins_upto (\<I>_it k inp) (Suc k) 0) = set_bins_upto (\<I>_it k inp) (Suc k) 0"
       unfolding \<pi>_step_def Scan_def Complete_def Predict_def bin_def by blast
-    also have "... \<subseteq> set_bins (\<I>_it k)"
+    also have "... \<subseteq> set_bins (\<I>_it k inp)"
       using wf Suc.prems set_bins_upto_sub_set_bins wf_bins_def by (metis length_bins_\<I>_it)
     finally show ?thesis .
   qed
-  have sound: "sound_items (set_bins (\<I>_it k))"
+  have sound: "sound_items inp (set_bins (\<I>_it k inp))"
     using Suc sound_\<I> \<I>_it_sub_\<I> by (metis Suc_lessD subset_antisym)
-  have "\<I> (Suc k) \<subseteq> \<pi> (Suc k) (set_bins (\<I>_it k))"
+  have "\<I> (Suc k) inp \<subseteq> \<pi> (Suc k) inp (set_bins (\<I>_it k inp))"
     using Suc \<pi>_sub_mono by simp
-  also have "... \<subseteq> set_bins (\<pi>_it (Suc k) (\<I>_it k))"
+  also have "... \<subseteq> set_bins (\<pi>_it (Suc k) inp (\<I>_it k inp))"
     using \<pi>_sub_\<pi>_it wf sub sound Suc.prems by simp
   finally show ?case
     by simp
@@ -1372,33 +1376,33 @@ qed
 
 lemma \<II>_sub_\<II>_it:
   assumes "set inp \<subseteq> set \<TT>"
-  shows "\<II> \<subseteq> set_bins \<II>_it"
+  shows "\<II> inp \<subseteq> set_bins (\<II>_it inp)"
   using assms \<I>_sub_\<I>_it \<II>_def \<II>_it_def by simp
 
 subsection \<open>Correctness\<close>
 
-definition earley_recognized_it :: "bool" where
-  "earley_recognized_it = (\<exists>x \<in> set (items (bins \<II>_it ! length inp)). is_finished x)"
+definition earley_recognized_it :: "'a sentence \<Rightarrow> bool" where
+  "earley_recognized_it inp = (\<exists>x \<in> set (items (bins (\<II>_it inp) ! length inp)). is_finished inp x)"
 
 theorem earley_recognized_it_iff_earley_recognized:
   assumes "set inp \<subseteq> set \<TT>"
-  shows "earley_recognized_it \<longleftrightarrow> earley_recognized"
+  shows "earley_recognized_it inp \<longleftrightarrow> earley_recognized inp"
 proof -
-  have "earley_recognized_it = (\<exists>x \<in> set (items (bins \<II>_it ! length inp)). is_finished x)"
+  have "earley_recognized_it inp = (\<exists>x \<in> set (items (bins (\<II>_it inp) ! length inp)). is_finished inp x)"
     unfolding earley_recognized_it_def by blast
-  also have "... = (\<exists>x \<in> set_bins \<II>_it. is_finished x)"
+  also have "... = (\<exists>x \<in> set_bins (\<II>_it inp). is_finished inp x)"
     using is_finished_def kth_bin_in_bins \<II>_it_def length_bins_Init_it length_bins_\<I>_it wf_bins_\<II>_it
       wf_item_in_kth_bin set_bin_def by (metis One_nat_def lessI less_add_same_cancel1 subset_code(1))
-  also have "... = (\<exists>x \<in> \<II>. is_finished x)"
-    using assms \<II>_it_sub_\<II> \<II>_sub_\<II>_it by auto
-  also have "... = earley_recognized"
+  also have "... = (\<exists>x \<in> \<II> inp. is_finished inp x)"
+    using assms \<II>_it_sub_\<II> \<II>_sub_\<II>_it by blast
+  also have "... = earley_recognized inp"
     unfolding earley_recognized_def by blast
   finally show ?thesis .
 qed
 
 corollary correctness_list:
   assumes "set inp \<subseteq> set \<TT>"
-  shows "earley_recognized_it \<longleftrightarrow> derives [\<SS>] inp"
+  shows "earley_recognized_it inp \<longleftrightarrow> derives [\<SS>] inp"
   using assms correctness earley_recognized_it_iff_earley_recognized by blast
 
 end
